1. Acceleration is constant, starting speed is $V_{x0}$, so
$$V_x = a*t + V_{0}$$

2. The starting position is $X_0$. The change in position is the area under the velocity graph: 

$$X(t) = \int V_x \, dt + X_{0}$$

$$X(t) = \int (a*t + V_{0}) \, dt + X_{0}$$

$$X(t) = \frac{1}{2} * a * t^2 + V_{x0} * t + X_{0}$$

3. Eliminating t

$$V_x = a*t + V_{0}$$

$$t = \frac{V_x - V_{0}}{a}$$

Sub into:

$$x = \frac{1}{2} * a * t^2+ v_{x0} * t + x_{0}$$

$$x = \frac{1}{2} * a * (\frac{v_x - v_{0}}{a})^2+ v_{x0} * \frac{v_x - v_{0}}{a} + x_{0}$$

$$x = \frac{a}{2} * \frac{(v_x - v_{0})^2}{a^2}+ v_{x0} * \frac{v_x - v_{0}}{a} + x_{0}$$

$$x = \frac{1}{2} * \frac{(v_x - v_{0})^2}{a}+ \frac{v_{x0} * v_x - v_{x0} * v_{0}}{a} + x_{0}$$

$$x = \frac{1}{2} * \frac{(v_x - v_{0})^2}{a}+ \frac{v_{x0} * v_x}{a} - \frac{v_{x0} * v_{0}}{a} + x_{0}$$

$$2ax = (v_x - v_{0})^2 + 2 * v_{x0} * v_x - 2 * v_{x0} * v_{0} + 2ax_{0}$$

$$2ax = v_x^2 - 2*v_x * v_{0} + v_{0}^2 + 2 * v_{x0} * v_x - 2 * v_{x0}^2 + 2ax_{0}$$

$$v_x^2 = 2ax + 2*v_x * v_{0} - v_{0}^2 - 2 * v_{x0} * v_x + 2 * v_{x0}^2 - 2ax_{0}$$

$$v_x^2 = 2ax  + v_{x0}^2 - 2ax_{0}$$

$$v_x^2 = v_{x0}^2 + 2a(x - x_{0})$$